generalized simulation theorems for arbitrary models

fairness/heap_lang/simulation_adequacy.v
@@ -1,7 +1,7 @@
 From stdpp Require Import fin_maps.
 From iris.proofmode Require Import tactics.
 From trillium.program_logic Require Export weakestpre adequacy.
-From trillium.fairness Require Export fairness.
+From trillium.fairness Require Export fairness traces_match.
 From trillium.fairness.heap_lang Require Export lang heap_lang_defs.
 
 Definition heap_lang_extrace : Type := extrace heap_lang.
@@ -59,4 +59,111 @@ Section adequacy.
     iModIntro. iFrame.
   Qed.
 
+  Theorem strong_simulation_adequacy_inftraces Σ
+
+    `{hPre: @heapGpreS Σ M EM} (s: stuckness) 
+    (e1 : expr) σ1 (s1: M)
+    (R: execution_trace heap_lang → auxiliary_trace M → Prop)
+    (p: em_init_param)
+    (iex : inf_execution_trace heap_lang)
+    (Hvex : valid_inf_exec (trace_singleton ([e1], σ1)) iex)
+    :
+    rel_finitary R →
+    em_is_init_st ([e1], σ1) s1 ->
+    (wp_premise Σ s e1 σ1 s1 R p) ->
+    exists iatr,
+      @valid_inf_system_trace _ M
+        (@continued_simulation
+           heap_lang
+           M
+           R)
+        (trace_singleton ([e1], σ1))
+        (trace_singleton s1)
+        iex
+        iatr.
+  Proof.
+    intros Hfin Hwp.
+    eexists.
+    eapply produced_inf_aux_trace_valid_inf.
+    Unshelve.
+    - econstructor.
+    - eapply (strong_simulation_adequacy_general s) => //.
+    - done.
+  Qed.
+
+  Definition FOO {M: Model}: extrace heap_lang -> trace (mstate M) (mlabel M) -> Prop.
+  Admitted.
+
+  (* TODO: move *)
+  Definition to_trace_trfirst {S L : Type}
+    (s: S) (il: inflist (L * S)):
+    trfirst (to_trace s il) = s.
+  Proof. 
+    destruct il as [| [??]]; done.
+  Qed. 
+
+  Theorem strong_simulation_adequacy_traces Σ
+    `{hPre: @heapGpreS Σ M EM} (s: stuckness) 
+    (e1 : expr) σ1 (s1: M)
+    (R: execution_trace heap_lang → auxiliary_trace M → Prop)
+    (p: em_init_param)
+
+    (extr : heap_lang_extrace)
+    (Hvex : extrace_valid extr)
+    (Hexfirst : trfirst extr = ([e1], σ1))
+
+    (valid_step: cfg heap_lang -> olocale heap_lang → cfg heap_lang → 
+                 mstate M → mlabel M → mstate M -> Prop)
+    (state_rel: cfg heap_lang -> mstate M -> Prop)
+    (lbl_rel: olocale heap_lang -> mlabel M -> Prop)
+    (STEP_LBL_REL: forall c1 oζ c2 δ1 ℓ δ2,
+                 valid_step c1 oζ c2 δ1 ℓ δ2 ->
+                 lbl_rel oζ ℓ)
+    (STEP_MTRANS: forall c1 oζ c2 δ1 ℓ δ2,
+                 valid_step c1 oζ c2 δ1 ℓ δ2 ->
+                 mtrans δ1 ℓ δ2)
+    (R_ST: forall extr mtr, R extr mtr -> state_rel (trace_last extr) (trace_last mtr))
+    (R_STEP: forall extr mtr, R extr mtr -> valid_state_evolution_fairness valid_step extr mtr)
+
+    :
+    rel_finitary R →
+    em_is_init_st ([e1], σ1) s1 ->
+    (wp_premise Σ s e1 σ1 s1 R p) ->
+    ∃ (mtr : trace (mstate M) (mlabel M)), 
+      traces_match lbl_rel state_rel locale_step (@mtrans M) extr mtr /\
+      trfirst mtr = s1. 
+  Proof.
+    intros Hfin INIT Hwp.
+    have [iatr Hbig] : exists iatr,
+        @valid_inf_system_trace
+          heap_lang M
+          (@continued_simulation
+             heap_lang
+             M
+             R)
+          (trace_singleton ([e1], (trfirst extr).2))
+          (trace_singleton s1)
+          (from_trace extr)
+          iatr.
+    { eapply (strong_simulation_adequacy_inftraces _ s); eauto.
+      eapply from_trace_preserves_validity; eauto; first econstructor.
+      all: by rewrite Hexfirst. }
+    exists (to_trace s1 iatr).
+    split.
+    2: { by rewrite to_trace_trfirst. }
+    
+    unshelve eapply (valid_inf_system_trace_implies_traces_match
+                       valid_step                       
+                       state_rel
+                       lbl_rel
+                       ltac:(idtac)
+                       ltac:(idtac)
+                       (continued_simulation R)); eauto.
+    - intros ?? ?%continued_simulation_rel. eauto.
+    - intros ?? ?%continued_simulation_rel. eauto.
+    - apply from_trace_spec. simpl.
+      rewrite Hexfirst. done. 
+    - apply to_trace_spec. 
+  Qed.
+  
 End adequacy.
